examples/ecommerce/EcommerceFixedCorrect.v
@@ -1,0 +1,438 @@
+From ConCert.Examples.Ecommerce Require Import EcommerceFixed.
+From ConCert.Execution Require Import BuildUtils.
+From ConCert.Utils Require Import Automation.
+From Coq Require Import ZArith.
+
+From ConCert.Execution Require Import Serializable.
+Require Import Blockchain.
+Require Import Containers.
+Require Import Extras.
+From ConCert.Utils Require Import RecordUpdate.
+From Coq Require Import Bool.
+From Coq Require Import Lia.
+From Coq Require Import List.
+Import ListNotations.
+
+Section Theories.
+
+Context `{Base : ChainBase}. 
+
+Arguments hash_bid : simpl never.
+Arguments hash_purchaseId : simpl never.
+
+Ltac receive_simpl_step g :=
+  match type of g with
+  | context[find_purchase] => unfold find_purchase in g; cbn in g
+  | context[find_item] => unfold find_item in g; cbn in g
+  | context[purchase_exists] => unfold purchase_exists in g; cbn in g
+  | context[FMap.find _ ?v] => destruct (FMap.find _ v) eqn:?; cbn in g
+  | context[setter_from_getter_State_purchases] => unfold setter_from_getter_State_purchases in g; cbn in g
+  | context[set_State_purchases] => unfold set_State_purchases in g; cbn in g
+  | context[setter_from_getter_Purchase_last_block] => unfold setter_from_getter_Purchase_last_block in g; cbn in g
+  | context[set_Purchase_last_block] => unfold set_Purchase_last_block in g; cbn in g
+  | context[setter_from_getter_Purchase_purchase_state] => unfold setter_from_getter_Purchase_purchase_state in g; cbn in g
+  | context[set_Purchase_purchase_state] => unfold set_Purchase_purchase_state in g; cbn in g
+  | context[setter_from_getter_Purchase_seller_bit] => unfold setter_from_getter_Purchase_seller_bit in g; cbn in g
+  | context[set_Purchase_seller_bit] => unfold set_Purchase_seller_bit in g; cbn in g
+  | context[required_true ?cond] => destruct cond eqn:?E; inversion E; cbn in g
+  end. 
+
+Tactic Notation "receive_simpl" constr(g) := cbn in g; repeat (receive_simpl_step g); try discriminate.
+
+Ltac receive_simpl_goal_step :=
+  match goal with
+  | |- context[find_purchase] => unfold find_purchase
+  | |- context[find_item] => unfold find_item
+  | |- context[purchase_exists] => unfold purchase_exists
+  | |- context[purchase_state_eq] => unfold purchase_state_eq
+  | |- context[setter_from_getter_State_purchases] => unfold setter_from_getter_State_purchases
+  | |- context[set_State_purchases] => unfold set_State_purchases
+  | |- context[setter_from_getter_Purchase_last_block] => unfold setter_from_getter_Purchase_last_block
+  | |- context[set_Purchase_last_block] => unfold set_Purchase_last_block
+  | |- context[setter_from_getter_Purchase_purchase_state] => unfold setter_from_getter_Purchase_purchase_state
+  | |- context[set_Purchase_purchase_state] => unfold set_Purchase_purchase_state
+  | |- context[setter_from_getter_Purchase_seller_bit] => unfold setter_from_getter_Purchase_seller_bit
+  | |- context[set_Purchase_seller_bit] => unfold set_Purchase_seller_bit
+  end. 
+
+Tactic Notation "receive_simpl_goal" := cbn; repeat (receive_simpl_goal_step; cbn).
+
+Open Scope Z.
+  
+Lemma purchase_state_eq_correct : forall (state1 state2 : PurchaseState),
+  state1 = state2 <-> purchase_state_eq state1 state2 = true.
+Proof.
+  intros *. split; intros; destruct state1; destruct state2; try discriminate; reflexivity.
+Qed.
+
+Lemma buyer_request_purchase_contract_correct : forall chain ctx prev_state new_state new_acts _itemId _notes,
+  EcommerceFixed.receive chain ctx prev_state (Some (buyer_request_purchase _itemId _notes)) = Some (new_state, new_acts)
+  <->
+     (exists item,
+         FMap.find _itemId prev_state.(listings) = Some item
+      /\ FMap.find _itemId new_state.(listings) = Some item
+      /\ item.(item_value) = ctx.(ctx_amount))
+  /\ (exists purchaseId new_purchase,
+         purchaseId = hash_purchaseId chain.(current_slot) (ctx.(ctx_from))
+      /\ FMap.find purchaseId prev_state.(purchases) = None
+      /\ new_state.(purchases) = FMap.add purchaseId new_purchase prev_state.(purchases)
+      /\ new_purchase.(itemId) = _itemId
+      /\ new_purchase.(last_block) = chain.(current_slot)
+      /\ new_purchase.(purchase_state) = requested
+      /\ new_purchase.(buyer) = ctx.(ctx_from)
+      /\ new_purchase.(seller_bit) = false
+      /\ new_purchase.(commit) = 0%N
+      /\ new_purchase.(notes) = _notes)
+  /\ prev_state.(listings) = new_state.(listings)
+  /\ prev_state.(seller) = new_state.(seller)
+  /\ prev_state.(timeout) = new_state.(timeout)
+  /\ new_acts = []
+  .
+Proof.
+  intros * . split.
+  - intros receive_some.
+    receive_simpl receive_some.
+    remember ({|
+    commit := 0;
+    last_block := current_slot
+      chain;
+    itemId := _itemId;
+    seller_bit := false;
+    notes := _notes;
+    purchase_state := requested;
+    buyer := ctx_from ctx |})
+    as new_purchase.
+    repeat split; try now inversion receive_some.
+    + exists i. repeat split; try now inversion receive_some.
+      now apply Z.eqb_eq in E.
+    + remember (hash_purchaseId chain.(current_slot) ctx.(ctx_from)) as new_purchaseId.
+      exists new_purchaseId, new_purchase.
+      repeat split; try now inversion Heqnew_purchase.
+      now inversion receive_some.
+  - intros ([item (prev_item & new_item & amount_sent)] &
+            (purchaseId & new_purchase & purchaseId_hash & not_found_purchase & purchase_added & purchase_itemId & purchase_last_block &
+             ppurchase_state & purchase_buyer & purchase_seller_bit & purchase_commit & purchase_notes) &
+             const_listings & const_seller & const_timeout & empty_acts).
+    receive_simpl_goal.
+    setoid_rewrite prev_item.
+    apply Z.eqb_eq in amount_sent. rewrite amount_sent; cbn.
+    rewrite <- purchaseId_hash.
+    setoid_rewrite not_found_purchase; cbn.
+    rewrite empty_acts.
+    rewrite const_listings, const_seller, const_timeout.
+    rewrite <- purchase_last_block, <- purchase_commit, <- purchase_itemId, <- purchase_seller_bit,
+            <- purchase_notes, <- ppurchase_state, <- purchase_buyer.   
+    destruct new_purchase; destruct new_state; cbn in *.
+    now setoid_rewrite <- purchase_added. 
+Qed.
+
+Lemma seller_accept_contract_correct : forall chain ctx prev_state new_state new_acts id,
+  EcommerceFixed.receive chain ctx prev_state (Some (seller_accept_contract id)) = Some (new_state, new_acts)
+  <->
+     (exists purchase updated_purchase,
+        FMap.find id prev_state.(purchases) = Some purchase
+      /\ purchase.(purchase_state) = requested
+      /\ FMap.find id new_state.(purchases) = Some updated_purchase
+      /\ updated_purchase.(purchase_state) = accepted
+      /\ updated_purchase.(last_block) = chain.(current_slot)
+      /\ updated_purchase.(commit) = purchase.(commit)
+      /\ updated_purchase.(itemId) = purchase.(itemId)
+      /\ updated_purchase.(seller_bit) = purchase.(seller_bit)
+      /\ updated_purchase.(notes) = purchase.(notes)
+      /\ updated_purchase.(buyer) = purchase.(buyer)
+      /\ new_state.(purchases) = FMap.add id updated_purchase prev_state.(purchases))
+  /\ (ctx.(ctx_from) =? prev_state.(seller) = true)%address
+  /\ prev_state.(listings) = new_state.(listings)
+  /\ prev_state.(seller) = new_state.(seller)
+  /\ prev_state.(timeout) = new_state.(timeout)
+  /\ new_acts = [].
+Proof.
+  intros *. split.
+  - intros receive_some. cbn in *.
+    receive_simpl receive_some.
+    remember ({|
+      commit := commit p;
+      last_block := current_slot chain;
+      itemId := itemId p;
+      seller_bit := seller_bit p;
+      notes := notes p;
+      purchase_state := accepted;
+      buyer := buyer p |})
+    as updated_purchase.
+    inversion receive_some; clear receive_some. cbn. repeat split.
+    exists p, updated_purchase. repeat split; try now inversion Hequpdated_purchase.
+    + now apply purchase_state_eq_correct in E.
+    + apply FMap.find_add.
+  - intros ([purchase [updated_purchase (purchase_found & state_requested & updated_purchase_found &
+                updated_state_accepted & block_current & commit_constant & item_constant &
+                seller_bit_constant & notes_constant & buyer_constant & purchase_added)]] &
+             ctx_from_seller & listings_constant & seller_constant & timeout_constant & no_acts).
+    receive_simpl_goal.
+    setoid_rewrite purchase_found.
+    rewrite state_requested; cbn.
+    rewrite ctx_from_seller; cbn.
+    rewrite no_acts; cbn.
+    rewrite seller_constant, listings_constant, timeout_constant.
+    rewrite <- updated_state_accepted, <- block_current, <- commit_constant, <- item_constant,
+            <- seller_bit_constant, <- notes_constant, <- buyer_constant.
+            auto.
+    destruct updated_purchase; destruct new_state; cbn in *.
+    now setoid_rewrite <- purchase_added.
+Qed.
+
+Lemma buyer_dispute_delivery_correct : forall chain ctx prev_state new_state new_acts id commitment,
+  EcommerceFixed.receive chain ctx prev_state (Some (buyer_dispute_delivery id commitment)) = Some (new_state, new_acts)
+  <->
+  (exists purchase updated_purchase item,
+     FMap.find id prev_state.(purchases) = Some purchase
+  /\ (ctx.(ctx_from) =? purchase.(buyer))%address = true
+  /\ purchase.(purchase_state) = delivered
+  /\ FMap.find purchase.(itemId) prev_state.(listings) = Some item
+  /\ (ctx.(ctx_amount) =? item.(item_value)) = true
+  /\ updated_purchase.(purchase_state) = dispute
+  /\ updated_purchase.(last_block) = chain.(current_slot)
+  /\ new_state.(purchases) = FMap.add id updated_purchase prev_state.(purchases)
+  (* These fields should stay constant *)
+  /\ commitment = updated_purchase.(commit)
+  /\ purchase.(itemId) = updated_purchase.(itemId)
+  /\ purchase.(seller_bit) = updated_purchase.(seller_bit)
+  /\ purchase.(notes) = updated_purchase.(notes)
+  /\ purchase.(buyer) = updated_purchase.(buyer))
+  /\ prev_state.(listings) = new_state.(listings)
+  /\ prev_state.(seller) = new_state.(seller)
+  /\ prev_state.(timeout) = new_state.(timeout)
+  
+  /\ new_acts = []
+  .
+Proof.
+  intros *. split.
+  - intros receive_some.
+    receive_simpl receive_some.
+    remember ({|
+    commit := commitment;
+    last_block := current_slot chain;
+    itemId := itemId p;
+    seller_bit := seller_bit p;
+    notes := notes p;
+    purchase_state := dispute;
+    buyer := buyer p |})
+    as updated_purchase.
+    repeat split; try now inversion receive_some.
+    exists p, updated_purchase, i.
+    repeat split; try now inversion Hequpdated_purchase.
+    + now apply purchase_state_eq_correct in E.
+    + now inversion receive_some.
+  - intros ([purchase [updated_purchase [item 
+            (purchase_found & purchase_from & state_delivered & item_found & item_val & upd_purchase_from & block_current & upd_purchases & com & const_item & const_seller_bit & const_notes & const_buyer)
+  ]]] & const_listings & const_seller & const_timeout & acts_empty).
+  receive_simpl_goal.
+  setoid_rewrite purchase_found.
+  rewrite state_delivered, purchase_from; cbn.
+  setoid_rewrite item_found.
+  rewrite item_val; cbn.
+  rewrite acts_empty.
+
+  rewrite const_item, const_seller_bit, const_notes, const_buyer,
+          const_listings, const_seller, const_timeout,
+          com, <- upd_purchase_from, <- block_current.
+  destruct updated_purchase; destruct new_state;
+  now setoid_rewrite <- upd_purchases.
+Qed.
+
+Lemma buyer_open_commitment_correct : forall chain ctx prev_state new_state new_acts id buyer_bit nonce,
+  EcommerceFixed.receive chain ctx prev_state (Some (buyer_open_commitment id buyer_bit nonce)) = Some (new_state, new_acts)
+  <->
+  (exists purchase updated_purchase _item,
+     FMap.find id prev_state.(purchases) = Some purchase
+  /\ FMap.find id new_state.(purchases) = Some updated_purchase
+  /\ FMap.find purchase.(itemId) prev_state.(listings) = Some _item
+  /\ new_state.(purchases) = FMap.add id updated_purchase prev_state.(purchases)
+  (* Only state should change in the targeted purchase *)
+  /\ failed = updated_purchase.(purchase_state)
+  /\ purchase.(last_block) = updated_purchase.(last_block)
+  /\ purchase.(commit) = updated_purchase.(commit)
+  /\ purchase.(itemId) = updated_purchase.(itemId)
+  /\ purchase.(seller_bit) = updated_purchase.(seller_bit)
+  /\ purchase.(notes) = updated_purchase.(notes)
+  /\ purchase.(buyer) = updated_purchase.(buyer)
+  
+  /\ purchase.(purchase_state) = counter
+  /\ hash_bid id buyer_bit nonce = purchase.(commit)
+  /\ (ctx.(ctx_from) =? purchase.(buyer))%address = true
+  /\ (eqb purchase.(seller_bit) buyer_bit = true
+     -> new_acts = [act_transfer purchase.(buyer) (2*_item.(item_value))])
+  /\ (eqb purchase.(seller_bit) buyer_bit = false
+     -> new_acts = [act_transfer prev_state.(seller) (2*_item.(item_value))])
+  )
+  /\ prev_state.(listings) = new_state.(listings)
+  /\ prev_state.(seller) = new_state.(seller)
+  /\ prev_state.(timeout) = new_state.(timeout)
+  .
+  intros *. split.
+  - intros receive_some.
+    receive_simpl receive_some.
+    remember ({|
+    commit := commit p;
+    last_block := last_block p;
+    itemId := itemId p;
+    seller_bit := seller_bit p;
+    notes := notes p;
+    purchase_state := failed;
+    buyer := buyer p |})
+    as updated_purchase.
+    repeat split; try now inversion Hequpdated_purchase; try now inversion receive_some.
+    exists p, updated_purchase, i.
+    repeat split; try now inversion Hequpdated_purchase.
+    + inversion receive_some; cbn. apply FMap.find_add.
+    + now inversion receive_some.
+    + now apply purchase_state_eq_correct in E0.
+    + now apply N.eqb_eq in E1.
+    + intros eq_bits. inversion receive_some. rewrite eq_bits. now rewrite H0.
+    + intros neq_bits. inversion receive_some. now rewrite neq_bits. 
+  - intros ([purchase [updated_purchase [_item
+            (purchase_found & updated_purchase_found & item_found & purchases_updated & upd_purchase_failed &
+             const_block & const_commit & const_item & const_seller_bit & const_notes & const_buyer &
+             purchase_counter & correct_hash & ctx_from_buyer & eq_bits & neq_bits)]]] &
+             const_listings & const_seller & const_timeout).
+    receive_simpl_goal.
+    setoid_rewrite purchase_found.
+    rewrite ctx_from_buyer; cbn.
+    rewrite purchase_counter; cbn.
+    apply N.eqb_eq in correct_hash; rewrite correct_hash; cbn.
+    setoid_rewrite item_found.
+    rewrite const_seller, const_listings, const_timeout.
+    rewrite const_commit, const_block, const_item,
+            const_seller_bit,const_notes, const_buyer.
+    rewrite upd_purchase_failed.
+    destruct updated_purchase; destruct new_state; cbn in *. auto.
+    setoid_rewrite <- purchases_updated.  
+    rewrite const_seller_bit in eq_bits, neq_bits.
+    destruct (eqb seller_bit buyer_bit) eqn:E.
+    + rewrite eq_bits; easy.
+    + rewrite neq_bits; easy.
+Qed.
+
+Lemma seller_item_was_delivered_correct : forall chain ctx prev_state new_state new_acts id,
+  EcommerceFixed.receive chain ctx prev_state (Some (seller_item_was_delivered id)) = Some (new_state, new_acts)
+  <->
+  (exists purchase updated_purchase,
+      FMap.find id prev_state.(purchases) = Some purchase
+   /\ FMap.find id new_state.(purchases) = Some updated_purchase
+   /\ new_state.(purchases) = FMap.add id updated_purchase prev_state.(purchases)
+   /\ purchase.(purchase_state) = accepted
+   /\ updated_purchase.(purchase_state) = delivered
+   /\ updated_purchase.(last_block) = chain.(current_slot)
+   (* These should remain constant *)
+   /\ purchase.(commit) = updated_purchase.(commit)
+   /\ purchase.(itemId) = updated_purchase.(itemId)
+   /\ purchase.(seller_bit) = updated_purchase.(seller_bit)
+   /\ purchase.(notes) = updated_purchase.(notes)
+   /\ purchase.(buyer) = updated_purchase.(buyer))
+  /\ prev_state.(listings) = new_state.(listings)
+  /\ prev_state.(seller) = new_state.(seller)
+  /\ prev_state.(timeout) = new_state.(timeout)
+
+  /\ (ctx.(ctx_from) =? prev_state.(seller))%address = true
+  /\ new_acts = []
+  .
+Proof.
+  intros *. split.
+  - intros receive_some.
+    receive_simpl receive_some.
+    repeat split; try now inversion receive_some.
+    remember ({|
+    commit := commit p;
+    last_block := current_slot chain;
+    itemId := itemId p;
+    seller_bit := seller_bit p;
+    notes := notes p;
+    purchase_state := delivered;
+    buyer := buyer p |})
+    as updated_purchase.
+    exists p, updated_purchase.
+    repeat split; try now inversion Hequpdated_purchase; try now inversion receive_some.
+    + inversion receive_some; cbn. apply FMap.find_add.
+    + now inversion receive_some.
+    + now apply purchase_state_eq_correct in E.
+  - intros ([purchase [updated_purchase
+            (found_purchase & found_upd_purchase & purchases_updated & purchase_accepted & upd_purchase_delivered & upd_purchase_block &
+             const_commit & const_item & const_seller_bit & const_notes & const_buyer)]] &
+            const_listings & const_seller & const_timeout & from_seller & empty_acts).
+    receive_simpl_goal.
+    setoid_rewrite found_purchase.
+    rewrite purchase_accepted, from_seller; cbn.
+    rewrite const_seller, const_listings, const_timeout.
+    rewrite const_commit, const_item, const_notes, const_seller_bit, const_buyer.
+    rewrite <- upd_purchase_delivered, <- upd_purchase_block, empty_acts.
+    destruct updated_purchase; destruct new_state; cbn.
+    now setoid_rewrite purchases_updated.
+Qed.
+
+Lemma seller_counter_dispute : forall chain ctx prev_state new_state new_acts id random_bit,
+  EcommerceFixed.receive chain ctx prev_state (Some (seller_counter_dispute id random_bit)) = Some (new_state, new_acts)
+  <->
+  (exists purchase updated_purchase item,
+      FMap.find id prev_state.(purchases) = Some purchase
+   /\ FMap.find id new_state.(purchases) = Some updated_purchase
+   /\ FMap.find purchase.(itemId) prev_state.(listings) = Some item
+   /\ new_state.(purchases) = FMap.add id updated_purchase prev_state.(purchases)
+   /\ purchase.(purchase_state) = dispute
+   /\ updated_purchase.(seller_bit) = random_bit
+   /\ updated_purchase.(purchase_state) = counter
+   /\ updated_purchase.(last_block) = chain.(current_slot)
+   /\ ctx.(ctx_amount) = item.(item_value)
+   (* These should remain constant *)
+   /\ purchase.(commit) = updated_purchase.(commit)
+   /\ purchase.(itemId) = updated_purchase.(itemId)
+   /\ purchase.(notes) = updated_purchase.(notes)
+   /\ purchase.(buyer) = updated_purchase.(buyer))
+  /\ prev_state.(listings) = new_state.(listings)
+  /\ prev_state.(seller) = new_state.(seller)
+  /\ prev_state.(timeout) = new_state.(timeout)
+
+  /\ (ctx.(ctx_from) =? prev_state.(seller))%address = true
+  /\ new_acts = []
+.
+Proof.
+  intros *. split.
+  - intros receive_some.
+    receive_simpl receive_some.
+    repeat split; try now inversion receive_some.
+    unfold setter_from_getter_Purchase_seller_bit in *.
+    unfold set_Purchase_seller_bit in *.
+    remember ({|
+    commit := commit p;
+    last_block := current_slot chain;
+    itemId := itemId p;
+    seller_bit := random_bit;
+    notes := notes p;
+    purchase_state := counter;
+    buyer := buyer p |})
+    as updated_purchase.
+    exists p, updated_purchase, i.
+    repeat split; try now inversion Hequpdated_purchase.
+    + inversion receive_some; cbn. apply FMap.find_add.
+    + now inversion receive_some.
+    + now apply purchase_state_eq_correct in E.
+    + now apply Z.eqb_eq in E1.
+  - intros ([purchase [updated_purchase [item (
+             found_purchase & found_upd_purchase & found_item & updated_purchases & purchase_dispute &
+             seller_bit_rand & upd_purchase_counter & upd_purchase_block & amount_as_item &
+             const_commit & const_item & const_notes & const_buyer
+            )]]] &
+            const_listings & const_seller & const_timeout & from_seller & empty_acts).
+    receive_simpl_goal.
+    setoid_rewrite found_purchase.
+    rewrite purchase_dispute; cbn.
+    rewrite from_seller; cbn.
+    rewrite empty_acts.
+    setoid_rewrite found_item.
+    apply Z.eqb_eq in amount_as_item; rewrite amount_as_item; cbn.
+    rewrite const_seller, const_listings, const_timeout.
+    rewrite const_commit, <- upd_purchase_block, <- seller_bit_rand, <- upd_purchase_counter,
+            const_item, const_notes, const_buyer.
+    destruct updated_purchase; destruct new_state; cbn.
+    now setoid_rewrite <- updated_purchases. 
+Qed.
+
+End Theories.
